\documentclass{article}
\usepackage[margin=0.5in]{geometry}
\usepackage[utf8]{inputenc}
\usepackage{euler}
\usepackage{amsfonts}
\usepackage{amsmath}
\usepackage{amssymb}
\usepackage{enumitem}
\usepackage{float}
\let\emptyset\varnothing

\author{Otavio Macedo}
\title{A Book of Abtract Algebra - solutions to exercises}


\begin{document}

\maketitle

\section*{Chapter 2}
\subsection*{Set A}
\begin{enumerate}
\item $a * b = \sqrt{|ab|}$ on the set $\mathbb{Q}$. This is not an operation on $\mathbb{Q}$. Square roots have two real solutions, some of them irrational. So, this operation is neither unique nor closed under $\mathbb{Q}$.

\item $a * b = a \ln b$, on the set ${x \in \mathbb{R}},\ x > 0$. This is not an operation because it's not closed. For instance, if $b = 1$ then $a\ln b = 0$, which does not belong to the set above.

\item $a * b$ is a root of the equation $x^2 - a^2b^2 = 0$, on the set $\mathbb{R}$. This is not an operation, since $a * b = \pm ab$, hence not unique.

\item Subtraction, on the set $\mathbb{Z}$. This is an operation.

\item Subtraction, on the set ${n \in \mathbb{Z} : n \geq 0}$. This is not an operation, since a subtraction of non-negative integers may result in a negative integer (not closed under the set).

\end{enumerate}

\subsection*{Set B}

\begin{enumerate}
\item $x * y = x + 2y + 4$. Commutative: no; Associative: no; Identity: no; Inverses: no.
\begin{enumerate}[label=(\roman*)]
    \item $0 * 1 = 6$ and $1 * 0 = 5$.
    \item $x * (y * z) = x + 2y + 4z + 12$. $(x * y) * z = x + 2y + 2z + 4$.
    \item $x * e = x \Rightarrow x + 2e + 4 = x \Rightarrow 2e + 4 = 0 \Rightarrow e = -2$. But this value of $e$ does not satisfy the equation $e * y = y$, since $-2 * y = -2 + 2y + 4 = 2y + 2 \ne y$.
    \item No identity implies no inverses.
\end{enumerate}

\item $x * y = x + 2y - xy$. Commutative: no; Associative: no; Identity: no; Inverses: no.
\begin{enumerate}[label=(\roman*)]
    \item $0 * 1 = 2$ and $1 * 0 = 1$.
    \item $(x * y) * z = 2y - xy - 2z - 2yz + xyz$ and $x * (y * z) = x + 2y + 4z - 2yz - xy - 2xz + xyz$.
    \item $x * e = x \Rightarrow x + 2e - xe = x \Rightarrow 2e - xe = 0 \Rightarrow e = 0$. But this value of $e$ does not satisfy the equation $e * y = y$, since $0 * y = 2y \ne y$.
    \item No identity implies no inverses.
\end{enumerate}

\item $x * y = |x + y|$.  Commutative: yes; Associative: no; Identity: yes; Inverses: yes.
\begin{enumerate}[label=(\roman*)]
    \item $|x + y| = |y + x|$.
    \item $||1 + -3| + -5| = 3$. But $|1 + |-3 + -5|| = 9$.
    \item $x * e = x \Rightarrow |x + e| = x \Rightarrow e = 0$. Being commutative, $x * e = e * x$. So $0$ is the identity.
    \item $x * x' = 0 \Rightarrow |x + x'| = 0 \Rightarrow x' = -x$. So, the inverse of $x$ is $-x$.
\end{enumerate}

\item $x * y = |x - y|$.   Commutative: yes; Associative: no; Identity: yes; Inverses: yes.
\begin{enumerate}[label=(\roman*)]
    \item $x - y = -(y - x) \Rightarrow |x - y| = |-(y - x)| = |y - x|$.
    \item $||1 - 3| - 5| = 3$. But $|1 - |3 - 5|| = 1$.
    \item $x * e = x \Rightarrow |x - e| = x \Rightarrow e = 0$. Being commutative, $x * e = e * x$. So $0$ is the identity.
    \item $x * x' = 0 \Rightarrow |x - x'| = 0 \Rightarrow x' = x$. So every element is its own inverse.
\end{enumerate}

\item $x * y = xy + 1$. Commutative: yes; Associative: no; Identity: no; Inverses: no.
\begin{enumerate}[label=(\roman*)]
    \item $xy + 1 = yx + 1$.
    \item $(x * y) * z = xyz + z + 1$. But $x * (y * z) = xyz + x + 1$.
    \item $x * e = x \Rightarrow xe + 1 = x$, which does not have a real solution.
    \item No identity implies no inverses.
\end{enumerate}

\item $x * y = \max\ \{x, y\}$. Commutative: yes; Associative: yes; Identity: no; Inverses: no.
\begin{enumerate}[label=(\roman*)]
    \item $\max\ \{x, y\} = \max\ \{y, x\}$.
    \item $\max\ \{x, \max\ \{y, z\}\} = \max\ \{\max\ \{x, y\}, z\}$.
    \item $x * e = x$ would imply that there exists an $e$ that is smaller than any $x \in \mathbb{R}$, which is false.
    \item No identity implies no inverses.
\end{enumerate}
\end{enumerate}

\subsection*{Set C}
Table \ref{tab:binary-operations} list all the operations for the set $\{a, b\}$. 

\begin{table}[]
    \centering
    \caption{Operations on $\{a, b\}$}
    \label{tab:binary-operations}
    \begin{tabular}{ll|llllllllllllllll}
    $x$ & $y$ & $O_1$ & $O_2$ & $O_3$ & $O_4$ & $O_5$ & $O_6$ & $O_7$ & $O_8$ & $O_9$ & $O_{10}$ & $O_{11}$ & $O_{12}$ & $O_{13}$ & $O_{14}$ & $O_{15}$ & $O_{16}$ \\
    $a$ & $a$ & $a$     & $a$     & $a$     & $a$     & $a$     & $a$     & $a$     & $a$     & $b$     & $b$      & $b$      & $b$      & $b$      & $b$      & $b$      & $b$      \\
    $a$ & $b$ & $a$     & $a$     & $a$     & $a$     & $b$     & $b$     & $b$     & $b$     & $a$     & $a$      & $a$      & $a$      & $b$      & $b$      & $b$      & $b$      \\
    $b$ & $a$ & $a$     & $a$     & $b$     & $b$     & $a$     & $a$     & $b$     & $b$     & $a$     & $a$      & $b$      & $b$      & $a$      & $a$      & $b$      & $b$      \\
    $b$ & $b$ & $a$     & $b$     & $a$     & $b$     & $a$     & $b$     & $a$     & $b$     & $a$     & $b$      & $a$      & $b$      & $a$      & $b$      & $a$      & $b$     
    \end{tabular}
\end{table}

\begin{enumerate}
    \item Commutative: $\{O_1, O_2, O_7, O_8, O_9, O_{10}, O_{15}, O_{16}\}$.
    \item Associative: $\{O_1, O_2, O_4, O_6, O_7, O_8, O_{10}, O_{16}\}$.
    \item Identity: $\{O_2, O_7, O_8, O_{10}\}$.
    \item Inverses: $\{O_7, O_{10}\}$.
\end{enumerate}

\subsection*{Set D}
\begin{enumerate}
    \item Let $a, b, c \in A^*$. Then:
        $$(ab)c = (a_1\ldots a_mb_1\ldots b_n)c_1\ldots c_p = a_1\ldots a_m(b_1\ldots b_nc_1\ldots c_p) = a(bc)$$
    \item Let $A = \{0, 1\}$ and $a = 001$ and $b = 110$, $a, b \in A^*$. Then $ab = 001110$ and $ba = 110001$, clearly showing that $ab \ne ba$.
    \item Let $a\lambda = \lambda a = a$. So $\lambda$ is the identity for this operation.
\end{enumerate}

\section*{Chapter 3}

\subsection*{Set A}

\begin{enumerate}
    \item $x * y = x + y + k$. Same thing as the example in Set B of Chapter 2, but with a generic constant $k$ instead of the fixed constant 1.
    \item $x * y = \frac{xy}{2}$, on the set $\{x \in \mathbb{R}, x \ne 0\}$.
    \begin{description}
        \item [Commutative] 
            $$\frac{xy}{2} = \frac{yx}{2}$$
        \item [Associative]
        $$(x * y) * z = \frac{xy}{2} * z = \frac{\frac{xy}{2}z}{2} = \frac{xyz}{4}$$
        $$x * (y * z) = \frac{x(y * z)}{2} = \frac{x\frac{yz}{2}}{2} = \frac{xyz}{4}$$
        \item [Identity] $x * e = x \Rightarrow \frac{xe}{2} = x \Rightarrow e = 2$
        \item [Inverse] $x * x' = 2 \Rightarrow \frac{xx'}{2} = 2 \Rightarrow xx' = 4 \Rightarrow x' = \frac{4}{x}$
    \end{description}
    \item $x * y = x + y + xy$, on the set $\{x \in \mathbb{R}, x \ne -1\}$
    \begin{description}
        \item [Commutative] $x + y + xy = y + x + yx$
        \item [Associative]
        $$(x * y) * z = (x + y + xy) * z = (x + y + xy) + x + (x + y + xy)z = x + y + z + xy + yz + xyz$$
        $$x * (y * z) = x * (y + z + yz) = x + (y + z + yz) + x(y + z + yz) = x + y + z + xy + yz + xyz$$
        \item [Identity] $x * e = x \Rightarrow x + e + xe = x \Rightarrow x + e + xe - x = 0 \Rightarrow x(1 + e - 1) + e = 0 \Rightarrow xe + e = 0 \Rightarrow e = 0$
        \item [Inverse] $x * x' = 0 \Rightarrow x + x'+ xx' = 0 \Rightarrow x = -x'(1 + x) \Rightarrow x' = \frac{x}{1+x}$
    \end{description}
    \item $x * y = \frac{x + y}{xy + 1}$, on the set $\{x \in \mathbb{R}, -1 < x < 1\}$.
    \begin{description}
        \item [Commutative]
            $$\frac{x + y}{xy + 1} = \frac{y + x}{yx + 1}$$
        \item [Associative]
            $$(x * y) * z = \frac{x + y}{xy + 1} * z = \frac{\left(\frac{x + y}{xy + 1}\right) + z}{\left(\frac{x + y}{xy + 1}\right)z + 1} = \frac{x + y + xyz + z}{xz + yz + xy + 1}$$
            $$x * (y * z) = x * \frac{y + z}{yz + 1} = \frac{x + \left(\frac{y + z}{yz + 1}\right)}{x\left(\frac{y + z}{yz + 1}\right) + 1} = \frac{x + y + xyz + z}{xz + yz + xy + 1}$$
        \item [Identity] $e * x = x * e = x \Rightarrow \frac{x + e}{xe + 1} = x \Rightarrow x + e = x(xe + 1) \Rightarrow e = 0$
        \item [Inverse] $x' * x = x * x' = 0 \Rightarrow \frac{x + x'}{xx' + 1} = 0 \Rightarrow x + x' = 0 \Rightarrow x' = -x$
    \end{description}
\end{enumerate}

\subsection*{Set B}
\begin{enumerate}
    \item $(a, b) * (c , d) = (ad + bc, bd)$, on the set $\{(x, y) \in \mathbb{R} \times \mathbb{R}: y \ne 0\}$: abelian group.
        \begin{description}
            \item [Commutative: Yes] $(ad + bc, bd) = (cb + da, bd)$
            \item [Associative: Yes]
                $$[(a, b) * (c, d)] * (f, g) = (ad + bc, bd) * (f, g) = (adg + bcg + bdf, bdg)$$
                $$(a, b) * [(c, d) * (f, g)] = (a, b) * (cg + df, dg) = (adg + bcg + bdf, bdg)$$
            \item [Identity: Yes]
                \begin{equation*}
                    \begin{split}
                        (e_1, e_2) * (a, b) = (a, b) * (e_1, e_2) = (a, b) & \Rightarrow (ae_2 + be_1, be_2) = (a, b) \\
                                                                           & \Rightarrow  \begin{cases}
                                                                                                be_2 = b \Rightarrow e_2 = 1 \\
                                                                                                ae_2 + be_1 = a \Rightarrow be_1 = 0 \Rightarrow e_1 = 0
                                                                                          \end{cases} \\
                                                                           & \Rightarrow e = (0, 1)
                    \end{split}
                \end{equation*}
            \item [Inverse: Yes]
                \begin{equation*}
                    \begin{split}
                        (a', b') * (a, b) = (a, b) * (a', b') = (0, 1) & \Rightarrow (ab' + ba', bb') = (0, 1) \\
                                                                       & \Rightarrow \begin{cases}
                                                                                            bb' = 1 \Rightarrow b' = \frac{1}{b} \\
                                                                                            ab' + ba' = 0 \Rightarrow \frac{a}{b} + ba' = 0 \Rightarrow a' = -\frac{a}{b^2}
                                                                                     \end{cases} \\
                                                                       & \Rightarrow (a, b)' = \left(-\frac{a}{b^2}, \frac{1}{b}\right)
                    \end{split}
                \end{equation*}
        \end{description}
    \item $(a, b) * (c, d) = (ac, bc + d)$, on the set $\{(x, y) \in \mathbb{R} \times \mathbb{R}: x \ne 0\}$: non-abelian group.
        \begin{description}
            \item [Commutative: No] $(ac, bc + d) \ne (ca, da + b)$
            \item [Associative: Yes]
                $$[(a, b) * (c, d)] * (f, g) = (ac, bc + d) * (f, g) = (acf, bcf + df + g)$$
                $$[(a, b) * [(c, d) * (f, g)] = (a, b) * (cf, df + g) = (acf, bcf + df + g)$$
            \item [Identity: Yes]
                \begin{equation*}
                    \begin{split}
                        (a, b) * (e_1, e_2) = (a, b) & \Rightarrow (ae_1 + be_1, e_2) = (a, b) \\
                                                    & \Rightarrow  \begin{cases}
                                                                        ae_1 = a \Rightarrow e_1 = 1 \\
                                                                        be_1 + e2 = b \Rightarrow b + e_2 = b \Rightarrow e_2 = 0
                                                                   \end{cases} \\
                                                    & \Rightarrow e = (1, 0)
                    \end{split}
                \end{equation*}
                Not being commutative, we have to check the inverse order of the operands:
                    $$(1, 0) * (a, b) = (1a + 0a, b) = (a, b)$$
            \item [Inverse: Yes]
                \begin{equation*}
                    \begin{split}
                        (a, b) * (a', b') = (1, 0) & \Rightarrow (aa' + ba', b') = (1, 0) \\
                                                & \Rightarrow \begin{cases}
                                                                    aa' = 1 \Rightarrow a' = \frac{1}{a} \\
                                                                    ba' + b' = 0 \Rightarrow \frac{b}{a} + b' = 0 \Rightarrow b' = -\frac{b}{a}
                                                                \end{cases}
                    \end{split}
                \end{equation*}
                Not being commutative, we have to check the inverse order of the operands:
                    $$\left(\frac{1}{a}, -\frac{b}{a}\right) * (a, b) = \left(\frac{1}{a}a, -\frac{b}{a}a + b\right) = (1, 0)$$
        \end{description}
    \item Same operation as in part 2, but on the set $\mathbb{R} \times \mathbb{R}$: not a group. There is no solution for the identity element.
    \item $(a, b) * (c, d = (ac -bd, ad + bc)$, on the set $\mathbb{R} \times \mathbb{R}$, with the origin deleted: abelian group.
        \begin{description}
            \item [Commutative: Yes] $(ac - bd, ad + bc) = (ca - db, cb + da)$
            \item [Associative: Yes]
                $$[(a, b) * (c, d)] * (f, g) = (ac - bd, ad + bc) * (f, g) = (acf - bdf - adg - bcg, acg - bdg + adf + bcf)$$
                $$(a, b) * [(c, d) * (f, g)] = (a, b) * (cf - dg, cg + df) = (acf - adg - bcg - bdf, acg + adf + bcf - bdg)$$
            \item [Identity: Yes]
                \begin{equation*}
                    \begin{split}
                        (e_1, e_2) * (a, b) = (a, b) * (e_1, e_2) = (a, b) & \Rightarrow (ae_1 - be_2, ae_2 + be_1) = (a, b) \\
                                                                           & \Rightarrow  \begin{cases}
                                                                                ae_1 - be_2 = a \Rightarrow e_1 = \frac{a + be_2}{a} \Rightarrow e_1 = 1 \\
                                                                                be_2 + be_1 = b \Rightarrow ae_2 + b\left(\frac{a + be_2}{a}\right) = b \Rightarrow e_2 = 0
                                                                             \end{cases} \\
                                                                           & \Rightarrow e = (1, 0)
                    \end{split}
                \end{equation*}
            \item [Inverses: Yes]
            \begin{equation*}
                \begin{split}
                    (a', b') * (a, b) = (a, b) * (a', b') = (1, 0) & \Rightarrow (aa' - bb', ab' + ba') = (1, 0) \\
                                                                   & \Rightarrow \begin{cases}
                                                                                        ab' + ba' = 0 \Rightarrow b' = -\frac{ba'}{a} \Rightarrow b'= -\frac{ba}{a^3 + ab^2}\\
                                                                                        aa' - bb' = 1 \Rightarrow aa' + \frac{b^2a'}{a} = 1 \Rightarrow a'= \frac{a}{a^2 + b^2}
                                                                                 \end{cases}\\
                                                                   & \Rightarrow (a, b)' = \left(\frac{a}{a^2 + b^2}, -\frac{ba}{a^3 + ab^2}\right)
                \end{split}
            \end{equation*}
    \end{description}
    \item Consider the operation of the preceding problem on the set $\mathbb{R} \times \mathbb{R}$. Is this a group? Explain.\\
    This is not a group. The value for the identity is undefined.
\end{enumerate}

\subsection*{Set C}
\begin{enumerate}
    \item $e = \emptyset$, since $\emptyset + A = A + \emptyset = (A - \emptyset) \cup (\emptyset - A) = A \cup A = A$.
    \item $A' + A = A + A' = \emptyset \Rightarrow (A - A') \cup (A'- A) = \emptyset \cup \emptyset = \emptyset$.
    \item $P_D = \{\emptyset, \{a\}, \{b\}, \{c\}, \{a, b\}, \{a, c\}, \{b, c\}, \{a, b, c\}\}$. See table \ref{tab:powerset-op}.
    \begin{table}[!ht]
        \centering
        \begin{tabular}{l|llllllll}
        +             & $\emptyset$   & $\{a\}$       & $\{b\}$       & $\{c\}$       & $\{a, b\}$    & $\{a, c\}$    & $\{b, c\}$    & $D$ \\
        \hline
        $\emptyset$   & $\emptyset$   & $\{a\}$       & $\{b\}$       & $\{c\}$       & $\{a, b\}$    & $\{a, c\}$    & $\{b, c\}$    & $D$ \\
        $\{a\}$       & $\{a\}$       & $\emptyset$   & $\{a, b\}$    & $\{a, c\}$    & $\{b\}$       & $\{c\}$       & $D$           & $\{b, c\}$    \\
        $\{b\}$       & $\{b\}$       & $\{a, b\}$    & $\emptyset$   & $\{b, c\}$    & $\{a\}$       & $D$           & $\{c\}$       & $\{a, c\}$    \\
        $\{c\}$       & $\{c\}$       & $\{a, c\}$    & $\{b, c\}$    & $\emptyset$   & $D$           & $\{a\}$       & $\{b\}$       & $\{a, b\}$    \\
        $\{a, b\}$    & $\{a, b\}$    & $\{b\}$       & $\{a\}$       & $D$           & $\emptyset$   & $\{b, c\}$    & $\{a, c\}$    & $\{c\}$       \\
        $\{a, c\}$    & $\{a, c\}$    & $\{c\}$       & $D$           & $\{a\}$       & $\{b, c\}$    & $\emptyset$   & $\{a, b\}$    & $\{b\}$       \\
        $\{b, c\}$    & $\{b, c\}$    & $D$           & $\{c\}$       & $\{b\}$       & $\{a, c\}$    & $\{a, b\}$    & $\emptyset$   & $\{a\}$       \\
        $D$           & $D$           & $\{b, c\}$    & $\{a, c\}$    & $\{a, b\}$    & $\{c\}$       & $\{b\}$       & $\{a\}$       & $\emptyset$  
        \end{tabular}
        \caption{Operation table for $\langle P_D, + \rangle$}
        \label{tab:powerset-op}
    \end{table}
\end{enumerate}

\subsection*{Set D}
See Table \ref{tab:checkerboard} for the checkerboard game operation table. $I$ is the identity since $X * I = I * X= X$ for any $X \in G$, and every element has an inverse (itself).
\begin{table}[H]
    \centering
    \begin{tabular}{l|llll}
    $*$ & $I$ & $V$ & $H$ & $D$ \\ \hline
    $I$ & $I$ & $V$ & $H$ & $D$ \\
    $V$ & $V$ & $I$ & $D$ & $H$ \\
    $H$ & $H$ & $D$ & $I$ & $V$ \\
    $D$ & $D$ & $H$ & $V$ & $I$
    \end{tabular}
    \caption{Operation table for $\langle G, *\rangle$}
    \label{tab:checkerboard}
\end{table}

\subsection*{Set E}
See Table \ref{tab:coingame-op} for the coin game operation table. $I$ is the identity, since $X * I = I * X = X$, for every $X \in G$. 
In every line there is an entry with $I$, which means that every element has an inverse.
$\langle G, *\rangle$ is not commutative. For instance: $M_2 * M_4 \ne M_4 * M_2$.

% TODO Write the table for the coin game.
\end{document}
